apps/derive/tests/test_tag.v
@@ -25,6 +25,7 @@ Elpi derive.tag iota.
 Elpi derive.tag large.
 Elpi derive.tag prim_int.
 Elpi derive.tag prim_float.
+Elpi derive.tag prim_string.
 Elpi derive.tag fo_record.
 Elpi derive.tag pa_record.
 Elpi derive.tag pr_record.
